Fishy output of fault localization for the program in out.bpl

gravy/src/org/gravy/faultlocalization/InfeasibleCodeFaultLocalization.java
@@ -13,113 +13,201 @@ import org.gravy.prover.Prover;
 import org.gravy.prover.ProverExpr;
 import org.gravy.prover.ProverFactory;
 import org.gravy.prover.ProverResult;
+import org.gravy.util.JavaSourceLocation;
 import org.gravy.verificationcondition.AbstractTransitionRelation;
 import org.gravy.verificationcondition.FaultLocalizationTransitionRelation;
 
+import boogie.ProgramFactory;
+import boogie.ast.Attribute;
+import boogie.ast.NamedAttribute;
 import boogie.controlflow.BasicBlock;
 import boogie.controlflow.CfgAxiom;
 import boogie.controlflow.CfgProcedure;
+import boogie.controlflow.statement.CfgAssertStatement;
+import boogie.controlflow.statement.CfgAssumeStatement;
 import boogie.controlflow.statement.CfgStatement;
 
 /**
  * @author schaef
- *
+ * 
  */
 public class InfeasibleCodeFaultLocalization {
 
 	/**
-	 * Applies fault localization to a set of (not necessarily connected) infeasible blocks.
+	 * Applies fault localization to a set of (not necessarily connected)
+	 * infeasible blocks.
+	 * 
 	 * @param tr
 	 * @param infeasibleBlocks
 	 */
-	public static void localizeFaults(AbstractTransitionRelation tr, Set<BasicBlock> infeasibleBlocks) {
+	public static void localizeFaults(AbstractTransitionRelation tr,
+			Set<BasicBlock> infeasibleBlocks) {
 		LinkedList<HashSet<BasicBlock>> components = findConnectedComponents(infeasibleBlocks);
 		for (HashSet<BasicBlock> cmp : components) {
 			localizeFault(tr, cmp);
 		}
 	}
 
-	
 	/**
 	 * Applies fault localization to a set of connected infeasible blocks
+	 * 
 	 * @param tr
 	 * @param component
 	 */
-	public static HashMap<CfgStatement, ProverExpr> localizeFault(AbstractTransitionRelation tr, Set<BasicBlock> component) {		
-		//TODO: check if this contains a noverify tag and ignore it. 
-		
-		CfgProcedure slice = tr.getProcedure().computeSlice(getSubprog(component), tr.getProcedure().getRootNode());
-		
+	public static HashMap<CfgStatement, JavaSourceLocation> localizeFault(
+			AbstractTransitionRelation tr, Set<BasicBlock> component) {
+		// TODO: check if this contains a noverify tag and ignore it.
+		for (BasicBlock b : component) {
+			if (containsNamedAttribute(b, ProgramFactory.NoVerifyTag)) {
+				return new HashMap<CfgStatement, JavaSourceLocation>();
+			}
+		}
+
+		CfgProcedure slice = tr.getProcedure().computeSlice(
+				getSubprog(component), tr.getProcedure().getRootNode());
+
 		ProverFactory pf = new org.gravy.prover.princess.PrincessProverFactory();
 		Prover prover = pf.spawn();
 		prover.setConstructProofs(true);
-		FaultLocalizationTransitionRelation sliceTr = new FaultLocalizationTransitionRelation(slice, tr.getControlFlowFactory(), prover);
-		
+		FaultLocalizationTransitionRelation sliceTr = new FaultLocalizationTransitionRelation(
+				slice, tr.getControlFlowFactory(), prover);
+
 		int partition = 0;
-		
-//		prover.addAssertion(sliceTr.getEnsures());
-//	
-		for (Entry<CfgAxiom, ProverExpr> entry : sliceTr.getPreludeAxioms().entrySet()) {
+
+		// prover.addAssertion(sliceTr.getEnsures());
+		//
+		for (Entry<CfgAxiom, ProverExpr> entry : sliceTr.getPreludeAxioms()
+				.entrySet()) {
 			prover.addAssertion(entry.getValue());
 		}
-		
-		
+
 		prover.addAssertion(sliceTr.getRequires());
-		
+
 		prover.setPartitionNumber(partition++);
-        
-        for (ProverExpr assertion : sliceTr.obligations) {
-            prover.addAssertion(assertion);
-            prover.setPartitionNumber(partition++);        	
-        }
-		
+
+		for (ProverExpr assertion : sliceTr.obligations) {
+			prover.addAssertion(assertion);
+			prover.setPartitionNumber(partition++);
+		}
+
 		ProverResult res = prover.checkSat(true);
-		if (res!=ProverResult.Unsat) {
+		if (res != ProverResult.Unsat) {
 			throw new RuntimeException("Fault Localization failed!");
 		}
-		
 
-        int[][] ordering = new int[partition][1];
-        for (int i=0; i<partition; i++) {
-                ordering[i][0] = i;
-        }               
-        
+		int[][] ordering = new int[partition][1];
+		for (int i = 0; i < partition; i++) {
+			ordering[i][0] = i;
+		}
 
-        ProverExpr[] interpolants = prover.interpolate(ordering);
+		ProverExpr[] interpolants = prover.interpolate(ordering);
 
-        //debug code
-        {
-//                System.err.println("#interpolants: "+ interpolants.length + " / #assertions:");
-//                for (int i=0; i<partition-1; i++) {                        
-//                		System.err.println("Assertion "+i+":"+sliceTr.pe2StmtMap.get(sliceTr.obligations.get(i)));
-//                        System.err.println("\tInterpolant "+i+":"+interpolants[i]);
-//                }
-        }
-        
-        HashMap<CfgStatement, ProverExpr> interestingStatements = new HashMap<CfgStatement, ProverExpr>();
-        ProverExpr currentInterpolant = interpolants[0];
-        for (int i=1; i<interpolants.length; i++) {
-        	if (!interpolants[i].equals(currentInterpolant)) {
-        		currentInterpolant = interpolants[i];        		
-        		CfgStatement statement = sliceTr.pe2StmtMap.get(sliceTr.obligations.get(i));
-        		if (statement==null) {
-        			//TODO:
-        			statement = sliceTr.pe2StmtMap.get(sliceTr.obligations.get(i-1));
-        		}
-        		interestingStatements.put(statement, currentInterpolant);
-        		System.err.println("Interesting Stmt: ");
-        		System.err.println("\t"+statement);
-        		System.err.println("with interpolant: "+interpolants[i]);        		
-        	}
-        }
-        System.err.println("============");
-        
-        return interestingStatements;
+		// debug code
+		{
+			 System.err.println("#interpolants: "+ interpolants.length +
+			 " / #assertions:");
+			 for (int i=0; i<partition-1; i++) {
+			 System.err.println("Assertion "+i+":"+sliceTr.pe2StmtMap.get(sliceTr.obligations.get(i)));
+			 System.err.println("\tInterpolant "+i+":"+interpolants[i]);
+			 }
+		}
+
+		HashMap<CfgStatement, JavaSourceLocation> interestingStatements = new HashMap<CfgStatement, JavaSourceLocation>();
+		ProverExpr currentInterpolant = interpolants[0];
+		for (int i = 1; i < interpolants.length; i++) {
+			if (!interpolants[i].equals(currentInterpolant)) {
+				currentInterpolant = interpolants[i];
+				CfgStatement statement = sliceTr.pe2StmtMap
+						.get(sliceTr.obligations.get(i));
+				if (statement == null) {
+					// TODO:
+					statement = sliceTr.pe2StmtMap.get(sliceTr.obligations
+							.get(i - 1));
+				}
+
+				BasicBlock origin = sliceTr.stmtOriginMap.get(statement);
+				// if (origin==null || containsNamedAttribute(origin,
+				// ProgramFactory.Cloned)) {
+				// continue;
+				// }
+
+				JavaSourceLocation loc = null;
+
+				if (statement instanceof CfgAssertStatement
+						|| statement instanceof CfgAssumeStatement) {
+					if (statement instanceof CfgAssumeStatement
+							&& statement.getAttributes() == null
+							|| statement.getAttributes().length == 0) {
+						// this is a special case when a jar2bpl if statement is
+						// translated.
+						// probably not a good pick if the boogie file came from
+						// elsewhere.
+						int pos = origin.getStatements().indexOf(statement);
+						if (origin.getStatements().size()<=pos+1) {
+							pos--; //only if there is no further statement pick the 
+							//predecessor
+						} else {
+							pos++; //if its an assume without attribute
+							//pick the successor.
+						}
+						loc = praseLocationTags(origin.getStatements()
+								.get(pos).getAttributes());
+					} else {
+						loc = praseLocationTags(statement.getAttributes());
+					}
+				} else {
+					if (origin != null) {
+						int pos = origin.getStatements().indexOf(statement);
+						if (pos > 0
+								&& (origin.getStatements().get(pos - 1) instanceof CfgAssertStatement || origin
+										.getStatements().get(pos - 1) instanceof CfgAssumeStatement)) {
+							loc = praseLocationTags(origin.getStatements()
+									.get(pos - 1).getAttributes());
+						}
+					}
+				}
+				interestingStatements.put(statement, loc);
+				System.err.println("Interesting Stmt: ");
+				if (loc != null) {
+					System.err.print("l:" + loc.StartLine + "," + loc.StartCol);
+				}
+				System.err.println("\t" + statement);
+				System.err.println("with interpolant: " + interpolants[i]);
+			}
+		}
+		System.err.println("============");
+
+		prover.shutdown();
+
+		return interestingStatements;
 	}
-	
+
+	private static JavaSourceLocation praseLocationTags(Attribute[] attributes) {
+		if (attributes == null)
+			return null;
+		return JavaSourceLocation.readSourceLocationFromAttributes(attributes);
+	}
+
+	private static boolean containsNamedAttribute(BasicBlock b, String name) {
+		for (CfgStatement s : b.getStatements()) {
+			if (s.getAttributes() != null) {
+				for (Attribute attr : s.getAttributes()) {
+					if (attr instanceof NamedAttribute) {
+						NamedAttribute na = (NamedAttribute) attr;
+						if (na.getName().equals(name)) {
+							return true;
+						}
+					}
+				}
+			}
+		}
+		return false;
+	}
+
 	/**
-	 * Collect all blocks that must can reach or can be reached by
-	 * the elements in component 
+	 * Collect all blocks that must can reach or can be reached by the elements
+	 * in component
+	 * 
 	 * @param component
 	 * @return
 	 */
@@ -129,8 +217,9 @@ public class InfeasibleCodeFaultLocalization {
 		result.addAll(getNeighbors(component, false));
 		return result;
 	}
-	
-	private static Set<BasicBlock> getNeighbors(Set<BasicBlock> blocks, boolean forward) {
+
+	private static Set<BasicBlock> getNeighbors(Set<BasicBlock> blocks,
+			boolean forward) {
 		LinkedList<BasicBlock> todo = new LinkedList<BasicBlock>();
 		HashSet<BasicBlock> done = new HashSet<BasicBlock>();
 		todo.addAll(blocks);
@@ -145,43 +234,45 @@ public class InfeasibleCodeFaultLocalization {
 		}
 		return done;
 	}
-	
+
 	private static Set<BasicBlock> getNeighbors(BasicBlock b, boolean forward) {
-		if (forward) return b.getSuccessors();
+		if (forward)
+			return b.getSuccessors();
 		return b.getPredecessors();
 	}
-	
-	
-	private static LinkedList<HashSet<BasicBlock>> findConnectedComponents(Set<BasicBlock> blocks) {
+
+	private static LinkedList<HashSet<BasicBlock>> findConnectedComponents(
+			Set<BasicBlock> blocks) {
 		LinkedList<HashSet<BasicBlock>> components = new LinkedList<HashSet<BasicBlock>>();
 		LinkedList<BasicBlock> allblocks = new LinkedList<BasicBlock>();
 		allblocks.addAll(blocks);
 		while (!allblocks.isEmpty()) {
 			HashSet<BasicBlock> subprog = new HashSet<BasicBlock>();
 			LinkedList<BasicBlock> todo = new LinkedList<BasicBlock>();
-			todo.add(allblocks.pop());			
+			todo.add(allblocks.pop());
 
 			while (!todo.isEmpty()) {
 				BasicBlock current = todo.pop();
 				allblocks.remove(current);
 				subprog.add(current);
 				for (BasicBlock b : current.getPredecessors()) {
-					if (!subprog.contains(b) && !todo.contains(b) && allblocks.contains(b)) {
+					if (!subprog.contains(b) && !todo.contains(b)
+							&& allblocks.contains(b)) {
 						todo.add(b);
 					}
 				}
 				for (BasicBlock b : current.getSuccessors()) {
-					if (!subprog.contains(b) && !todo.contains(b) && allblocks.contains(b)) {
+					if (!subprog.contains(b) && !todo.contains(b)
+							&& allblocks.contains(b)) {
 						todo.add(b);
 					}
-				}				
-			}		
-			if (subprog.size()>0) {
+				}
+			}
+			if (subprog.size() > 0) {
 				components.add(subprog);
 			}
 		}
 		return components;
 	}
-	
 
 }
