gravy/src/org/gravy/report/InterpolationInfeasibleReport.java
@@ -1,0 +1,26 @@
+/**
+ * 
+ */
+package org.gravy.report;
+
+import java.util.Set;
+
+import org.gravy.faultlocalization.InfeasibleCodeFaultLocalization;
+import org.gravy.verificationcondition.AbstractTransitionRelation;
+
+import boogie.controlflow.AbstractControlFlowFactory;
+import boogie.controlflow.BasicBlock;
+
+/**
+ * @author schaef
+ *
+ */
+public class InterpolationInfeasibleReport extends Report {
+
+	public InterpolationInfeasibleReport(AbstractControlFlowFactory cff,
+			AbstractTransitionRelation tr, Set<BasicBlock> feasibleBlocks,
+			Set<BasicBlock> infeasibleBlocks) {
+		InfeasibleCodeFaultLocalization.localizeFaults(tr, infeasibleBlocks);
+	}	
+	
+}
